oPCF/Syntax.lean
@@ -1,3 +1,5 @@
+import «oPCF».Utility
+
 inductive Ty
   | bool
   | nat
@@ -13,10 +15,15 @@ infixl:100 " ∷ " => Cx.cons
 
 inductive Var : Cx → Ty → Type
   | z : Var (Γ ∷ τ) τ
-  | s : Var Γ τ → Var (Γ ∷ υ) τ
+  | s : ∀ τ, Var Γ τ → Var (Γ ∷ υ) τ
+
+def Var.succ (x : Var Γ τ) : Var (Γ ∷ υ) τ := s τ x
+
+def Var.tr_cx (t : Var Γ τ) : (Γ = Δ) → (Var Δ τ)
+  | p => by rw [p] at t; exact t
 
 inductive Tm : Cx → Ty → Type
-  | var : Var Γ τ → Tm Γ τ
+  | var : ∀ τ, Var Γ τ → Tm Γ τ
   | true : Tm Γ .bool
   | false : Tm Γ .bool
   | zero : Tm Γ .nat
@@ -29,6 +36,8 @@ inductive Tm : Cx → Ty → Type
   | fix : Tm Γ (τ ⇒ τ) → Tm Γ τ
 
 notation:10 Γ " ⊢ " τ => Tm Γ τ
+
+def Var.tm (x : Var Γ τ) : Γ ⊢ τ := Tm.var τ x
 
 def Tm.from_bool : Bool → (Γ ⊢ .bool)
   | .true => .true
@@ -45,54 +54,11 @@ inductive Tm.is_value : (Γ ⊢ τ) → Type
   | succ {v : Tm ..} : v.is_value → v.succ.is_value
   | fn {e : Tm ..} : e.fn.is_value
 
+def Cx.append (Γ : Cx) : Cx → Cx
+  | .nil => Γ
+  | .cons Δ τ => Γ.append Δ ∷ τ
 
-def Ren Γ Δ := ∀ {τ}, Var Γ τ → Var Δ τ
-def Reb Γ Δ := {τ : Ty} → Tm Γ τ → Tm Δ τ
-
-def extend_ren (r : Ren Γ Δ) {τ  : Ty} : Ren (Γ ∷ τ) (Δ ∷ τ) :=
-  fun v => match v with
-  | .z => .z
-  | .s x => .s (r x)
-
-def rename (r : Ren Γ Δ) : Reb Γ Δ :=
-  fun dv => match dv with
-  | .var x => .var (r x)
-  | .true => .true
-  | .false => .false
-  | .zero => .zero
-  | .succ e => (rename r e).succ
-  | .pred e => (rename r e).pred
-  | .zero? e => (rename r e).zero?
-  | .cond s et ef => (rename r s).cond (rename r et) (rename r ef)
-  | .fn e => (rename (extend_ren r) e).fn
-  | .app f a => (rename r f).app (rename r a)
-  | .fix f => (rename r f).fix
-
-def Tm.ren (t : Γ ⊢ τ) (r : Ren Γ Δ) : Δ ⊢ τ := rename r t
-
-def Subst Γ Δ := ∀ τ, Var Γ τ → Tm Δ τ
-
-def extend_subst (σ : Subst Γ Δ) {τ : Ty} : Subst (Γ ∷ τ) (Δ ∷ τ) :=
-  fun τ x => match x with
-  | .z => .var .z
-  | .s x => (σ τ x).ren .s
-
-def subst (σ : Subst Γ Δ) : Reb Γ Δ :=
-  fun {τ} e => match e with
-  | .var x => σ τ x
-  | .true => .true
-  | .false => .false
-  | .zero => .zero
-  | .succ e => (subst σ e).succ
-  | .pred e => (subst σ e).pred
-  | .zero? e => (subst σ e).zero?
-  | .cond s et ef => (subst σ s).cond (subst σ et) (subst σ ef)
-  | .fn e => (subst (extend_subst σ) e).fn
-  | .app f a => (subst σ f).app (subst σ a)
-  | .fix f => (subst σ f).fix
-
-def Tm.sub (t : Γ ⊢ τ) (σ : Subst Γ Δ) : Δ ⊢ τ := subst σ t
-
-def sb1 (a : Tm Γ υ) : Subst (Γ ∷ υ) Γ := fun τ v => match v with
-  | .z => a
-  | .s x => .var x
+def Cx.append_append_eq (Γ Δ₀ Δ₁ : Cx) : (Γ.append Δ₀).append Δ₁ = Γ.append (Δ₀.append Δ₁) := by
+  induction Δ₁ with
+  | nil => rfl
+  | cons Δ₁ τ Φ => calc ((Γ.append Δ₀).append Δ₁) ∷ τ = Γ.append (Δ₀.append Δ₁) ∷ τ := by rw [Φ]
