oPCF/Approximation.lean
@@ -1,0 +1,175 @@
+import «oPCF».Denotation
+import «oPCF».Operation
+
+-- NOTE: We define the type arguments of approximation in this order so τ can be inferred.
+-- Definition 27 (Formal approximation)
+def Approx : ∀ {τ}, (.nil ⊢ τ) → ↑⟦τ type⟧ → Type
+| .bool   => fun t d ↦ ∀ n,   d = .some n → t ⇓ Tm.from_bool n
+| .nat    => fun t d ↦ ∀ n,   d = .some n → t ⇓ Tm.from_nat n
+| .pow .. => fun t d ↦ ∀ u e, Approx u e → Approx (t.app u) (d e)
+
+infixl:75 " ▹ " => Approx
+notation:75 d " ◃ " t => Approx t d
+
+def Tm.approximations (t : .nil ⊢ τ) (d : ↑⟦τ type⟧) : Type := d ◃ t
+
+-- Definition 29 (Formal approximation for substitution)
+def Approx_Subst {Γ : Cx} (ρ : ⟦Γ cx⟧) (σ : Subst Γ .nil) : Type :=
+  ∀ τ x, ρ τ x ◃ σ τ x
+
+infixl:75 " ◃ " => Approx_Subst
+
+def from_nat_is_value : ∀ n, (Tm.from_nat n : Γ ⊢ .nat).is_value
+  | .zero => .zero
+  | .succ n => .succ (from_nat_is_value n)
+
+-- Lemma 31
+def bottom_approximates : ∀ {τ} {t : .nil ⊢ τ}, ⊥ ◃ t
+  | .bool   => fun _ p   ↦ Flat.noConfusion p
+  | .nat    => fun _ p   ↦ Flat.noConfusion p
+  | .pow .. => fun _ _ _ ↦ bottom_approximates
+
+-- Lemma 32
+noncomputable def supremum_approximates {τ} {t : .nil ⊢ τ} : ∀ {c}, (∀ n, c n ◃ t) → ⨆ c ◃ t := by
+  induction τ with
+  | bool | nat =>
+    intro c c_t d sc_d
+    have a := flat_sup_some.mpr sc_d
+    exact c_t a.choose d a.choose_spec
+  | pow τ₀ τ₁ _ Φ₁ =>
+    intro c c_t d u u_d
+    show ⨆ (c.apply u) ◃ t.app d
+    apply Φ₁
+    intro n
+    exact c_t n d u u_d
+
+-- Lemma 34
+noncomputable def same_eval_same_approx
+  : ∀ {t₀ t₁ : .nil ⊢ τ}, (∀ {v}, t₀ ⇓ v → t₁ ⇓ v) → ∀ {d}, (d ◃ t₀) → (d ◃ t₁) := by
+  intro t₀ t₁ same_eval d d_t₀
+  induction τ with
+  | bool | nat =>
+    intro n d_n
+    exact same_eval (d_t₀ n d_n)
+  | pow τ₀ τ₁ _ Φ₁ =>
+    intro u e e_u
+    have d_e_t₀_u : d e ◃ t₀.app u := d_t₀ u e e_u
+    show d e ◃ t₁.app u
+    suffices same_eval_app : ∀ {v}, t₀.app u ⇓ v → t₁.app u ⇓ v from Φ₁ same_eval_app d_e_t₀_u
+    intro v t₀_u_v
+    cases t₀_u_v with
+    | app f_fn_e e_u_v => exact .app (same_eval f_fn_e) e_u_v
+
+
+-- Theorem 29 (Fundamental property of formal approximation)
+noncomputable def approximation_fundamental {Γ : Cx} {ρ : ⟦Γ cx⟧} {σ : Subst Γ .nil} {t : Γ ⊢ τ}
+  : (ρ ◃ σ) → (⟦t⟧) ρ ◃ t.sub σ := by
+  induction t with
+  | var τ x =>
+    intro ρ_σ
+    exact ρ_σ τ x
+  | true | false | zero =>
+    intro _ _ h
+    injection h with h
+    rw [← h]
+    constructor
+  | app _ a Φf Φa =>
+    intro ρ_σ
+    exact Φf ρ_σ (a.sub σ) ((⟦a⟧) ρ) (Φa ρ_σ)
+  | succ t Φ =>
+    intro ρ_σ
+    suffices lem : ∀ {t : Tm ..} {d}, (d ◃ t) → (Cont.flat Nat.succ d ◃ t.succ) from lem (Φ ρ_σ)
+    intro t d d_t n succ_d_n
+    show t.succ ⇓ Tm.from_nat n
+    cases d with
+    | none => exact Flat.noConfusion succ_d_n
+    | some d =>
+      cases n with
+      | zero => injection succ_d_n with succ_d_0; exact Nat.noConfusion succ_d_0
+      | succ n =>
+        injection succ_d_n with h
+        injection h with d_n
+        rw [d_n] at d_t
+        exact .succ (d_t _ rfl)
+  | pred t Φ =>
+    intro ρ_σ
+    suffices lem : ∀ {t : Tm ..} {d}, (d ◃ t) → (Cont.flat Nat.pred d ◃ t.pred) from lem (Φ ρ_σ)
+    intro t d d_t n pred_d_n
+    show t.pred ⇓ Tm.from_nat n
+    cases d with
+    | none => exact Flat.noConfusion pred_d_n
+    | some d =>
+      injection pred_d_n with pred_d_n
+      cases d with
+      | zero =>
+        cases n with
+        | zero => exact .pred_zero (d_t 0 rfl)
+        | succ => injection pred_d_n
+      | succ d =>
+        change d = n at pred_d_n
+        rw [pred_d_n] at d_t
+        exact .pred_succ (from_nat_is_value n) (d_t n.succ rfl)
+  | zero? t Φ =>
+    intro ρ_σ
+    suffices lem : ∀ {t : Tm ..} {d}, (d ◃ t) → (Cont.flat Nat.zero? d ◃ t.zero?) from lem (Φ ρ_σ)
+    intro t d d_t n zero?_d_n
+    cases d with
+    | none => exact Flat.noConfusion zero?_d_n
+    | some d =>
+      injection zero?_d_n with zero?_d_n
+      cases d with
+      | zero =>
+        change true = n at zero?_d_n
+        rw [← zero?_d_n]
+        exact .zero?_zero (d_t .zero rfl)
+      | succ d =>
+        change false = n at zero?_d_n
+        rw [← zero?_d_n]
+        exact .zero?_succ (from_nat_is_value d) (d_t (d.succ) rfl)
+  | cond s t f Φs Φt Φf =>
+    intro ρ_σ
+    suffices lem : ∀ {s : Tm ..} {s'} {t f : Tm ..} {t' f'}, (s' ◃ s) → (t' ◃ t) → (f' ◃ f)
+      → Cont.cond.uncurry (s', (t', f')) ◃ s.cond t f
+      from lem (Φs ρ_σ) (Φt ρ_σ) (Φf ρ_σ)
+    intro s s' t f t' f' s'_s t'_t f'_f
+    cases s' with
+    | none =>
+      have h : Cont.cond.uncurry (Flat.none, t', f') = ⊥ := rfl
+      rw [h]
+      exact bottom_approximates
+    | some s' =>
+      cases s' with
+      | true =>
+        have same_eval : ∀ {v}, (t ⇓ v) → s.cond t f ⇓ v := fun t_v ↦ Eval.cond_true (s'_s true rfl) t_v
+        exact same_eval_same_approx same_eval t'_t
+      | false =>
+        have same_eval : ∀ {v}, (f ⇓ v) → s.cond t f ⇓ v := fun f_v ↦ Eval.cond_false (s'_s false rfl) f_v
+        exact same_eval_same_approx same_eval f'_f
+  | fix t Φ =>
+    intro ρ_σ
+    suffices lem : ∀ {t : Tm ..} {d}, (d ◃ t) → (Cont.fix d ◃ t.fix) from lem (Φ ρ_σ)
+    intro t d d_t
+    suffices closed : ∀ {e}, (e ◃ t.fix) → (d e ◃ t.fix)
+      from scott bottom_approximates supremum_approximates closed
+    intro e e_tfix
+    apply same_eval_same_approx Eval.fix
+    exact d_t t.fix e e_tfix
+  | @fn Δ τ υ e Φ =>
+    intro ρ_σ u d d_u
+    have tρd_tσu : (⟦e⟧) (ρ.push d) ◃ e.sub (σ.push u) := by {
+      apply Φ
+      show ρ.push d ◃ σ.push u
+      intro τ x
+      cases x with
+      | z => exact d_u
+      | s τ x => exact ρ_σ τ x
+    }
+    have same_eval : ∀ {v}, (e.sub (σ.push u) ⇓ v) → (e.fn.sub σ).app u ⇓ v := by {
+      intro v eσu_v
+      apply Eval.app Eval.fn
+      calc (e.sub (σ.keep _)).sub (Subst.inst u)
+        _ = e.sub (σ.keep _ ⬝ Subst.inst u) := by rw [sub_trans_eq]
+        _ = e.sub (σ.push u) := by rw [sub_push_eq_keep_inst]
+        _ ⇓ v := eσu_v
+    }
+    exact same_eval_same_approx same_eval tρd_tσu
