oPCF/Soundness.lean
@@ -2,8 +2,7 @@ import «oPCF».Denotation
 import «oPCF».Operation
 
 theorem eval_ground_bool : ∀ {n}, (⟦.from_bool n⟧) ρ = (.some n)
-  | .false => rfl
-  | .true => rfl
+  | .false | .true => rfl
 
 theorem eval_ground_nat : (⟦.from_nat n⟧) ρ = (.some n) := by
   induction n with
@@ -14,30 +13,36 @@ theorem eval_ground_nat : (⟦.from_nat n⟧) ρ = (.some n) := by
       _ = Cont.flat (.succ) (.some n)           := by rw [Φ]
       _ = .some (n.succ)                        := rfl
 
-theorem deno_ren_eq (e : Γ ⊢ τ) : ∀ Δ, (r : Ren Γ Δ) → ⟦e.ren r⟧ = (⟦e⟧) ∘' (⟦r⟧) := by
+theorem deno_ren_eq (e : Γ ⊢ τ) : ∀ {Δ}, (r : Ren Γ Δ) → ⟦e.ren r⟧ = (⟦e⟧) ∘' (⟦r⟧) := by
   induction e with
-  | var => intro Γ r; rfl
-  | true => intro _ _; rfl
-  | false => intro _ _ ; rfl
-  | zero => intro _ _; rfl
-  | succ t Φ =>
+  | fn e Φ =>
     intro _ r
-    calc ⟦t.succ.ren r⟧
-      _ = Cont.flat Nat.succ ∘' ⟦t.ren r⟧ := rfl
-      _ = Cont.flat Nat.succ ∘' (⟦t⟧) ∘' ⟦r⟧ := by rw [Φ _ r]
-      _ = (⟦t.succ⟧) ∘' ⟦r⟧ := rfl
-  | pred t Φ =>
-    intro _ r
-    calc ⟦t.pred.ren r⟧
-      _ = Cont.flat Nat.pred ∘' ⟦t.ren r⟧ := rfl
-      _ = Cont.flat Nat.pred ∘' (⟦t⟧) ∘' ⟦r⟧ := by rw [Φ _ r]
-      _ = (⟦t.pred⟧) ∘' ⟦r⟧ := rfl
-  | zero? t Φ =>
-    intro _ r
-    calc ⟦t.zero?.ren r⟧
-      _ = Cont.flat Nat.zero? ∘' ⟦t.ren r⟧ := rfl
-      _ = Cont.flat Nat.zero? ∘' (⟦t⟧) ∘' ⟦r⟧ := by rw [Φ _ r]
-      _ = (⟦t.zero?⟧) ∘' ⟦r⟧ := rfl
+    calc ⟦e.fn.ren r⟧
+      _ = Cont.curry ((⟦e.ren r.keep⟧) ∘ Ev.from) := rfl
+      _ = Cont.curry (((⟦e⟧) ∘' ⟦r.keep⟧) ∘ Ev.from) := by rw [Φ r.keep]
+      _ = (⟦e.fn⟧) ∘' ⟦r⟧ := by {
+        apply Cont.ext ∘ funext
+        intro ρ
+        apply Cont.ext ∘ funext
+        intro d
+        have p : (⟦r.keep⟧) (Ev.from (ρ, d)) = Ev.from ((⟦r⟧) ρ, d) := by {
+          apply funext
+          intro τ
+          apply funext
+          intro x
+          cases x with
+          | z => rfl
+          | s x => rfl
+        }
+        calc ((((⟦e⟧) ∘' ⟦r.keep⟧) ∘' Ev.from).curry ρ) d
+          _ = (⟦e⟧) ((⟦r.keep⟧) (Ev.from (ρ, d))) := rfl
+          _ = (⟦e⟧) (Ev.from ((⟦r⟧) ρ, d)) := by rw [p]
+          _ = ((⟦e.fn⟧) ((⟦r⟧) ρ)) d := rfl
+      }
+  | var | true | false | zero => intros; rfl
+  | succ _ Φ | pred _ Φ | zero? _ Φ | fix _ Φ => intro _ r; exact congrArg _ (Φ r)
+  | app f a Φf Φa =>
+    intro _ r; exact congrArg2 (fun f a ↦ Cont.eval ∘' Cont.pair f a) (Φf r) (Φa r)
   | cond s t f Φs Φt Φf =>
     intro _ r
     calc ⟦(s.cond t f).ren r⟧
@@ -47,42 +52,6 @@ theorem deno_ren_eq (e : Γ ⊢ τ) : ∀ Δ, (r : Ren Γ Δ) → ⟦e.ren r⟧ 
       _ = Cont.uncurry (Cont.cond) ∘' Cont.pair (⟦s⟧) ((Cont.pair (⟦t⟧) (⟦f⟧))) ∘' ⟦r⟧
         := by rw [Cont.pair_after (⟦t⟧) (⟦f⟧) (⟦r⟧), Cont.pair_after (⟦s⟧) _ (⟦r⟧)]
       _ = (⟦s.cond t f⟧) ∘' ⟦r⟧ := rfl
-  | fn e Φ =>
-    intro _ r
-    calc ⟦e.fn.ren r⟧
-      _ = Cont.curry ((⟦e.ren (extend_ren r)⟧) ∘ Ev.from) := rfl
-      _ = Cont.curry (((⟦e⟧) ∘' ⟦extend_ren r⟧) ∘ Ev.from) := by rw [Φ _ (extend_ren r)]
-      _ = (⟦e.fn⟧) ∘' ⟦r⟧ := by {
-        apply Cont.ext ∘ funext
-        intro ρ
-        apply Cont.ext ∘ funext
-        intro d
-        have p : (⟦extend_ren r⟧) (Ev.from (ρ, d)) = Ev.from ((⟦r⟧) ρ, d) := by {
-          apply funext
-          intro τ
-          apply funext
-          intro x
-          cases x with
-          | z => rfl
-          | s x => rfl
-        }
-        calc ((((⟦e⟧) ∘' ⟦extend_ren r⟧) ∘' Ev.from).curry ρ) d
-          _ = (⟦e⟧) ((⟦extend_ren r⟧) (Ev.from (ρ, d))) := rfl
-          _ = (⟦e⟧) (Ev.from ((⟦r⟧) ρ, d)) := by rw [p]
-          _ = ((⟦e.fn⟧) ((⟦r⟧) ρ)) d := rfl
-      }
-  | app f a Φf Φa =>
-    intro _ r
-    calc ⟦(f.app a).ren r⟧
-      _ = Cont.eval ∘' Cont.pair (⟦f.ren r⟧) (⟦a.ren r⟧) := rfl
-      _ = Cont.eval ∘' Cont.pair ((⟦f⟧) ∘' ⟦r⟧) ((⟦a⟧) ∘' ⟦r⟧) := by rw [Φf _ r, Φa _  r]
-      _ = (⟦f.app a⟧) ∘' ⟦r⟧ := rfl
-  | fix f Φ =>
-    intro _ r
-    calc ⟦f.fix.ren r⟧
-      _ = Cont.fix' ∘' ⟦f.ren r⟧ := rfl
-      _ = Cont.fix' ∘' (⟦f⟧) ∘' ⟦r⟧ := by rw [Φ _ r]
-      _ = (⟦f.fix⟧) ∘' ⟦r⟧ := rfl
 
 theorem ren_s_eq : (⟦.s⟧) (Ev.from (ρ, d)) = ρ := by
   apply funext
@@ -91,30 +60,42 @@ theorem ren_s_eq : (⟦.s⟧) (Ev.from (ρ, d)) = ρ := by
   intro x
   rfl
 
-theorem deno_subst_eq (e : Γ ⊢ τ) : ∀ Δ, (σ : Subst Γ Δ) → ⟦e.sub σ⟧ = (⟦e⟧) ∘' (⟦σ⟧) := by
+theorem deno_subst_eq (e : Γ ⊢ τ) : ∀ {Δ}, (σ : Subst Γ Δ) → ⟦e.sub σ⟧ = (⟦e⟧) ∘' (⟦σ⟧) := by
   induction e with
-  | var => intro _ _; rfl
-  | true => intro _ _; rfl
-  | false => intro _ _ ; rfl
-  | zero => intro _ _; rfl
-  | succ t Φ =>
+  | fn e Φ =>
     intro _ σ
-    calc ⟦t.succ.sub σ⟧
-      _ = Cont.flat Nat.succ ∘' ⟦t.sub σ⟧ := rfl
-      _ = Cont.flat Nat.succ ∘' (⟦t⟧) ∘' ⟦σ⟧ := by rw [Φ _ σ]
-      _ = (⟦t.succ⟧) ∘' ⟦σ⟧ := rfl
-  | pred t Φ =>
-    intro _ σ
-    calc ⟦t.pred.sub σ⟧
-      _ = Cont.flat Nat.pred ∘' ⟦t.sub σ⟧ := rfl
-      _ = Cont.flat Nat.pred ∘' (⟦t⟧) ∘' ⟦σ⟧ := by rw [Φ _ σ]
-      _ = (⟦t.pred⟧) ∘' ⟦σ⟧ := rfl
-  | zero? t Φ =>
-    intro _ σ
-    calc ⟦t.zero?.sub σ⟧
-      _ = Cont.flat Nat.zero? ∘' ⟦t.sub σ⟧ := rfl
-      _ = Cont.flat Nat.zero? ∘' (⟦t⟧) ∘' ⟦σ⟧ := by rw [Φ _ σ]
-      _ = (⟦t.zero?⟧) ∘' ⟦σ⟧ := rfl
+    calc ⟦e.fn.sub σ⟧
+      _ = Cont.curry ((⟦e.sub (σ.keep _)⟧) ∘ Ev.from) := rfl
+      _ = Cont.curry (((⟦e⟧) ∘' ⟦σ.keep _⟧) ∘ Ev.from) := by rw [Φ (σ.keep _)]
+      _ = (⟦e.fn⟧) ∘' ⟦σ⟧ := by {
+        apply Cont.ext ∘ funext
+        intro ρ
+        apply Cont.ext ∘ funext
+        intro d
+        have p : (⟦σ.keep _⟧) (Ev.from (ρ, d)) = Ev.from ((⟦σ⟧) ρ, d) := by {
+          apply funext
+          intro τ
+          apply funext
+          intro x
+          cases x with
+          | z => rfl
+          | s τ x =>
+            calc (⟦σ.keep _⟧) (Ev.from (ρ, d)) τ x.succ
+              _ = (⟦(σ τ x).ren .s⟧) (Ev.from (ρ, d)) := rfl
+              _ = ((⟦σ τ x⟧) ∘' ⟦.s⟧) (Ev.from (ρ, d)) := by rw [deno_ren_eq]
+              _ = (⟦σ τ x⟧) ((⟦.s⟧) (Ev.from (ρ, d))) := rfl
+              _ = (⟦σ τ x⟧) (ρ) := by rw [ren_s_eq]
+              _ = Ev.from ((⟦σ⟧) ρ, d) τ x.s := rfl
+        }
+        calc ((((⟦e⟧) ∘' ⟦σ.keep _⟧) ∘' Ev.from).curry ρ) d
+          _ = (⟦e⟧) ((⟦σ.keep _⟧) (Ev.from (ρ, d))) := rfl
+          _ = (⟦e⟧) (Ev.from ((⟦σ⟧) ρ, d)) := by rw [p]
+          _ = ((⟦e.fn⟧) ((⟦σ⟧) ρ)) d := rfl
+      }
+  | var | true | false | zero => intros; rfl
+  | succ _ Φ | pred _ Φ | zero? _ Φ | fix _ Φ => intro _ σ; exact congrArg _ (Φ σ)
+  | app _ _ Φf Φa =>
+    intro _ σ; exact congrArg2 (fun f a ↦ Cont.eval ∘' Cont.pair f a) (Φf σ) (Φa σ)
   | cond s t f Φs Φt Φf =>
     intro _ σ
     calc ⟦(s.cond t f).sub σ⟧
@@ -124,50 +105,9 @@ theorem deno_subst_eq (e : Γ ⊢ τ) : ∀ Δ, (σ : Subst Γ Δ) → ⟦e.sub 
       _ = Cont.uncurry (Cont.cond) ∘' Cont.pair (⟦s⟧) ((Cont.pair (⟦t⟧) (⟦f⟧))) ∘' ⟦σ⟧
         := by rw [Cont.pair_after (⟦t⟧) (⟦f⟧) (⟦σ⟧), Cont.pair_after (⟦s⟧) _ (⟦σ⟧)]
       _ = (⟦s.cond t f⟧) ∘' ⟦σ⟧ := rfl
-  | fn e Φ =>
-    intro _ σ
-    calc ⟦e.fn.sub σ⟧
-      _ = Cont.curry ((⟦e.sub (extend_subst σ)⟧) ∘ Ev.from) := rfl
-      _ = Cont.curry (((⟦e⟧) ∘' ⟦extend_subst σ⟧) ∘ Ev.from) := by rw [Φ _ (extend_subst σ)]
-      _ = (⟦e.fn⟧) ∘' ⟦σ⟧ := by {
-        apply Cont.ext ∘ funext
-        intro ρ
-        apply Cont.ext ∘ funext
-        intro d
-        have p : (⟦extend_subst σ⟧) (Ev.from (ρ, d)) = Ev.from ((⟦σ⟧) ρ, d) := by {
-          apply funext
-          intro τ
-          apply funext
-          intro x
-          cases x with
-          | z => rfl
-          | s x =>
-            calc (⟦extend_subst σ⟧) (Ev.from (ρ, d)) τ x.s
-              _ = (⟦(σ τ x).ren .s⟧) (Ev.from (ρ, d)) := rfl
-              _ = ((⟦σ τ x⟧) ∘' ⟦.s⟧) (Ev.from (ρ, d)) := by rw [deno_ren_eq]
-              _ = (⟦σ τ x⟧) ((⟦.s⟧) (Ev.from (ρ, d))) := rfl
-              _ = (⟦σ τ x⟧) (ρ) := by rw [ren_s_eq]
-              _ = Ev.from ((⟦σ⟧) ρ, d) τ x.s := rfl
-        }
-        calc ((((⟦e⟧) ∘' ⟦extend_subst σ⟧) ∘' Ev.from).curry ρ) d
-          _ = (⟦e⟧) ((⟦extend_subst σ⟧) (Ev.from (ρ, d))) := rfl
-          _ = (⟦e⟧) (Ev.from ((⟦σ⟧) ρ, d)) := by rw [p]
-          _ = ((⟦e.fn⟧) ((⟦σ⟧) ρ)) d := rfl
-      }
-  | app f a Φf Φa =>
-    intro _ σ
-    calc ⟦(f.app a).sub σ⟧
-      _ = Cont.eval ∘' Cont.pair (⟦f.sub σ⟧) (⟦a.sub σ⟧) := rfl
-      _ = Cont.eval ∘' Cont.pair ((⟦f⟧) ∘' ⟦σ⟧) ((⟦a⟧) ∘' ⟦σ⟧) := by rw [Φf _ σ, Φa _  σ]
-      _ = (⟦f.app a⟧) ∘' ⟦σ⟧ := rfl
-  | fix f Φ =>
-    intro _ σ
-    calc ⟦f.fix.sub σ⟧
-      _ = Cont.fix' ∘' ⟦f.sub σ⟧ := rfl
-      _ = Cont.fix' ∘' (⟦f⟧) ∘' ⟦σ⟧ := by rw [Φ _ σ]
-      _ = (⟦f.fix⟧) ∘' ⟦σ⟧ := rfl
 
-theorem deno_sb1_eq : ⟦sb1 a⟧ = Ev.from ∘' (Cont.pair Cont.id' (⟦a⟧)) := by
+-- Proposition 27 (Substitution property of the semantic function)
+theorem deno_inst_eq : ⟦Subst.inst a⟧ = Ev.from ∘' (Cont.pair Cont.id' (⟦a⟧)) := by
   apply Cont.ext ∘ funext
   intro d
   apply funext
@@ -175,18 +115,22 @@ theorem deno_sb1_eq : ⟦sb1 a⟧ = Ev.from ∘' (Cont.pair Cont.id' (⟦a⟧)) 
   apply funext
   intro x
   cases x with
-  | z => rfl
-  | s => rfl
+  | z | s => rfl
 
+-- Theorem 28 (Soundness)
 theorem soundness {t v : Cx.nil ⊢ τ} : t ⇓ v → ⟦t⟧ = ⟦v⟧ := by
   intro e
   induction e with
-  | true => rfl
-  | false => rfl
-  | zero => rfl
-  | succ _ t' => exact ap (λ p ↦ Cont.flat _ ∘' p) t'
-  | fn => rfl
-  | @pred v t _ _ t_v_succ =>
+  | true | false | zero | fn => rfl
+  | succ _ t_v => exact congrArg (fun p ↦ Cont.flat _ ∘' p) t_v
+  | @pred_zero t _ t_zero =>
+    apply Cont.ext ∘ funext
+    intro ρ
+    calc (⟦t.pred⟧) ρ
+      _ = Cont.flat (Nat.pred) ((⟦t⟧) ρ) := rfl
+      _ = Cont.flat (Nat.pred) ((⟦.zero⟧) ρ) := by rw [t_zero]
+      _ = (⟦.zero⟧) ρ := rfl
+  | @pred_succ v t _ _ t_v_succ =>
     apply Cont.ext ∘ funext
     intro ρ
     calc (⟦t.pred⟧) ρ
@@ -203,7 +147,7 @@ theorem soundness {t v : Cx.nil ⊢ τ} : t ⇓ v → ⟦t⟧ = ⟦v⟧ := by
     calc (⟦t.zero?⟧) ρ
       _ = Cont.flat (Nat.zero?) ((⟦t⟧) ρ) := rfl
       _ = Cont.flat (Nat.zero?) ((⟦Tm.zero⟧) ρ) := by rw [t_zero]
-      _ = (⟦Tm.true⟧) ρ := rfl
+      _ = (⟦.true⟧) ρ := rfl
   | @zero?_succ v t v' _ t_v_succ =>
     apply Cont.ext ∘ funext
     intro ρ
@@ -214,20 +158,20 @@ theorem soundness {t v : Cx.nil ⊢ τ} : t ⇓ v → ⟦t⟧ = ⟦v⟧ := by
       _ = Cont.flat (Nat.zero?) (Cont.flat .succ ((⟦v⟧) ρ)) := rfl
       _ = Cont.flat (Nat.zero?) (Cont.flat .succ ((⟦.from_nat n⟧) ρ)) := by rw [vn]
       _ = Cont.flat (Nat.zero?) (Cont.flat .succ (.some n)) := by rw [eval_ground_nat]
-      _ = (⟦Tm.false⟧) ρ := rfl
+      _ = (⟦.false⟧) ρ := rfl
   | @cond_true _ s t f tv _ _ se te =>
     apply Cont.ext ∘ funext
     intro ρ
     calc (⟦s.cond t f⟧) ρ
       _ = (Cont.cond ((⟦s⟧) ρ) ((⟦t⟧) ρ, (⟦f⟧) ρ)) := rfl
-      _ = (Cont.cond ((⟦Tm.true⟧) ρ) ((⟦tv⟧) ρ, (⟦f⟧) ρ)) := by rw [se, te]
+      _ = (Cont.cond ((⟦.true⟧) ρ) ((⟦tv⟧) ρ, (⟦f⟧) ρ)) := by rw [se, te]
       _ = (⟦tv⟧) ρ := rfl
   | @cond_false _ s t f fv _ _ se fe =>
     apply Cont.ext ∘ funext
     intro ρ
     calc (⟦s.cond t f⟧) ρ
       _ = (Cont.cond ((⟦s⟧) ρ) ((⟦t⟧) ρ, (⟦f⟧) ρ)) := rfl
-      _ = (Cont.cond ((⟦Tm.false⟧) ρ) ((⟦t⟧) ρ, (⟦fv⟧) ρ)) := by rw [se, fe]
+      _ = (Cont.cond ((⟦.false⟧) ρ) ((⟦t⟧) ρ, (⟦fv⟧) ρ)) := by rw [se, fe]
       _ = (⟦fv⟧) ρ := rfl
   | @app _ _ f a v e _ _ sf sv =>
     apply Cont.ext ∘ funext
@@ -236,8 +180,8 @@ theorem soundness {t v : Cx.nil ⊢ τ} : t ⇓ v → ⟦t⟧ = ⟦v⟧ := by
       _ = ((⟦f⟧) ρ) ((⟦a⟧) ρ) := rfl
       _ = ((⟦e.fn⟧) ρ) ((⟦a⟧) ρ) := by rw [sf]
       _ = ((⟦e⟧) ∘' Ev.from ∘' (Cont.pair Cont.id' (⟦a⟧))) ρ := rfl
-      _ = ((⟦e⟧) ∘' ⟦sb1 a⟧) ρ := by rw [deno_sb1_eq]
-      _ = (⟦e.sub (sb1 a)⟧) ρ := by rw [deno_subst_eq]
+      _ = ((⟦e⟧) ∘' ⟦Subst.inst a⟧) ρ := by rw [deno_inst_eq]
+      _ = (⟦e.sub (Subst.inst a)⟧) ρ := by rw [deno_subst_eq]
       _ = (⟦v⟧) ρ := by rw [sv]
   | @fix _ v f _ f_v =>
     apply Cont.ext ∘ funext
