oPCF/Substitution.lean
@@ -1,0 +1,355 @@
+import «oPCF».Syntax
+
+def Ren Γ Δ := ∀ τ, Var Γ τ → Var Δ τ
+def Reb Γ Δ := {τ : Ty} → Tm Γ τ → Tm Δ τ
+
+def Ren.trans (r₀₁ : Ren Γ₀ Γ₁) (r₁₂ : Ren Γ₁ Γ₂) : Ren Γ₀ Γ₂ :=
+  fun τ x => r₁₂ τ (r₀₁ τ x)
+
+instance : Trans Ren Ren Ren where
+  trans := Ren.trans
+
+def Ren.id' : Ren Γ Γ := fun _ ↦ id
+
+def Ren.weak {τ  : Ty} : Ren Γ (Γ ∷ τ) := Var.s
+
+def Ren.weaks : (Δ : Cx) → Ren Γ (Γ.append Δ)
+  | .nil => id'
+  | .cons Δ _ => fun υ x ↦ weak υ (weaks Δ υ x)
+
+def Ren.keep (r : Ren Γ Δ) {τ  : Ty} : Ren (Γ ∷ τ) (Δ ∷ τ) :=
+  fun υ v => match v with
+  | .z => .z
+  | .s τ x => .s τ (r τ x)
+
+def Ren.keeps (r : Ren Γ₀ Γ₁) : (Δ : Cx) → Ren (Γ₀.append Δ) (Γ₁.append Δ)
+  | .nil => r
+  | .cons Δ _ => (r.keeps Δ).keep
+
+theorem Ren.id_keep_eq_keep {Γ : Cx} (τ : Ty)
+  : Ren.id'.keep = (Ren.id' : Ren (Γ ∷ τ) (Γ ∷ τ)) := by
+  funext υ x
+  cases x with
+  | z | s => rfl
+
+theorem Ren.keeps_keep_eq_keep (r : Ren Γ₀ Γ₁) {Δ : Cx} (τ : Ty)
+  : (r.keeps Δ).keep = r.keeps (Δ ∷ τ) := by
+  funext υ x
+  rfl
+
+def Ren.swap {α β : Ty} : Ren (Γ ∷ β ∷ α) (Γ ∷ α ∷ β) := fun _ x ↦ match x with
+  | .z => .s α .z
+  | .s α .z => .z
+  | .s _ (.s _ x) => x.succ.succ
+
+def rename (r : Ren Γ Δ) : Reb Γ Δ :=
+  fun dv => match dv with
+  | .var τ x => .var τ (r τ x)
+  | .true => .true
+  | .false => .false
+  | .zero => .zero
+  | .succ e => (rename r e).succ
+  | .pred e => (rename r e).pred
+  | .zero? e => (rename r e).zero?
+  | .cond s et ef => (rename r s).cond (rename r et) (rename r ef)
+  | .fn e => (rename (r.keep) e).fn
+  | .app f a => (rename r f).app (rename r a)
+  | .fix f => (rename r f).fix
+
+def Tm.ren (t : Γ ⊢ τ) (r : Ren Γ Δ) : Δ ⊢ τ := rename r t
+
+def Tm.tr_cx (t : Γ ⊢ τ) (p : Γ = Δ) : (Δ ⊢ τ) :=
+  t.ren (fun _ x ↦ x.tr_cx p)
+
+def Tm.ren_id {t : Γ ⊢ τ} : t.ren Ren.id' = t := by
+  induction t with
+  | fn e Φ =>
+    calc (e.ren Ren.id'.keep).fn
+      _ = (e.ren Ren.id').fn := by rw [Ren.id_keep_eq_keep]
+      _ = e.fn := by rw [Φ]
+  | var | true | false | zero => intros; rfl
+  | succ e Φ | pred e Φ | zero? e Φ | fix e Φ => exact congrArg _ Φ
+  | app f a Φf Φa => exact congrArg2 _ Φf Φa
+  | cond s t f Φs Φt Φf => exact congrArg3 _ Φs Φt Φf
+
+def Tm.tr_cx_rfl (t : Γ ⊢ τ) : t.tr_cx rfl = t := by
+  exact Tm.ren_id
+
+theorem Ren.keep_composite_eq {r₀₁ : Ren Γ₀ Γ₁} {r₁₂ : Ren Γ₁ Γ₂}
+  : (r₀₁ ⬝ r₁₂).keep = (r₀₁.keep ⬝ r₁₂.keep : Ren (Γ₀ ∷ τ) (Γ₂ ∷ τ)) := by
+  funext τ x
+  cases x with | z | s => rfl
+
+theorem Ren.weak_after_eq {r : Ren Γ₀ Γ₁} : r ⬝ Ren.weak = (Ren.weak ⬝ r.keep : Ren Γ₀ (Γ₁ ∷ υ)) := by
+  funext τ x
+  rfl
+
+theorem ren_trans_eq {t : Γ₀ ⊢ τ}
+  : ∀ {Γ₁ Γ₂} {σ₀₁ : Ren Γ₀ Γ₁} {σ₁₂ : Ren Γ₁ Γ₂}, t.ren (σ₀₁ ⬝ σ₁₂) = (t.ren σ₀₁).ren σ₁₂ := by
+  induction t with
+  | @fn _ τ υ e Φ =>
+    intro _ _ r₀₁ r₁₂
+    calc (e.ren (r₀₁ ⬝ r₁₂).keep).fn
+      _ = (e.ren (r₀₁.keep ⬝ r₁₂.keep)).fn := by rw [Ren.keep_composite_eq]
+      _ = ((e.ren r₀₁.keep).ren r₁₂.keep).fn := by rw [Φ]
+  | var | true | false | zero => intros; rfl
+  | succ e Φ | pred e Φ | zero? e Φ | fix e Φ => exact congrArg _ Φ
+  | app f a Φf Φa => exact congrArg2 _ Φf Φa
+  | cond s t f Φs Φt Φf => exact congrArg3 _ Φs Φt Φf
+
+-- Definition 28 (Parallel closed substitution)
+def Subst Γ Δ := ∀ τ, Var Γ τ → Tm Δ τ
+
+-- TODO: Remove unused variants
+def Subst.keep (σ : Subst Γ Δ) (τ : Ty) : Subst (Γ ∷ τ) (Δ ∷ τ) :=
+  fun _ x => match x with
+  | .z => .var τ .z
+  | .s τ x => (σ τ x).ren .s
+
+def Subst.keeps' (σ : Subst Γ₀ Γ₁) : (Δ : Cx) → Subst (Γ₀.append Δ) (Γ₁.append Δ)
+  | .nil => σ
+  | .cons Δ τ => (σ.keeps' Δ).keep τ
+
+theorem Subst.keeps_keep_eq_keep (σ : Subst Γ₀ Γ₁) {Δ : Cx} (τ : Ty)
+  : (σ.keeps' Δ).keep τ = σ.keeps' (Δ ∷ τ) := by
+  funext υ x
+  rfl
+
+def subst (σ : Subst Γ Δ) : Reb Γ Δ :=
+  fun {τ} e => match e with
+  | .var _ x => σ τ x
+  | .true => .true
+  | .false => .false
+  | .zero => .zero
+  | .succ e => (subst σ e).succ
+  | .pred e => (subst σ e).pred
+  | .zero? e => (subst σ e).zero?
+  | .cond s et ef => (subst σ s).cond (subst σ et) (subst σ ef)
+  | .fn e => (subst (σ.keep _) e).fn
+  | .app f a => (subst σ f).app (subst σ a)
+  | .fix f => (subst σ f).fix
+
+def Tm.sub (t : Γ ⊢ τ) (σ : Subst Γ Δ) : Δ ⊢ τ := subst σ t
+
+def Subst.id' : Subst Γ Γ := fun τ x => .var τ x
+
+def Subst.trans (σ₀₁ : Subst Γ₀ Γ₁) (σ₁₂ : Subst Γ₁ Γ₂) : Subst Γ₀ Γ₂ :=
+  fun τ x => (σ₀₁ τ x).sub σ₁₂
+
+instance : Trans Subst Subst Subst where
+  trans := Subst.trans
+
+def Subst.inst : (t : Γ ⊢ τ) → Subst (Γ ∷ τ) Γ :=
+  fun a τ x => match x with
+  | .z => a
+  | .s τ x => .var τ x
+
+def Subst.amend (σ : Subst Γ₁ Γ₂) (r : Ren Γ₀ Γ₁) : Subst Γ₀ Γ₂ :=
+  fun τ x => σ τ (r τ x)
+
+def Subst.push (σ : Subst Γ Δ) {υ : Ty} (a : Δ ⊢ υ) : Subst (Γ ∷ υ) Δ :=
+  fun τ x => match x with
+  | .z => a
+  | .s τ x => σ τ x
+
+def Subst.weak {υ : Ty} : Subst Γ (Γ ∷ υ):=
+  fun _ x => x.succ.tm
+
+set_option pp.proofs true
+
+def id_keep_eq_id : (Subst.id' : Subst Γ Γ).keep τ = Subst.id' := by
+  funext τ x
+  cases x with | z | s => rfl
+
+def sub_id_eq {t : Γ ⊢ τ} : t.sub (Subst.id') = t := by
+  induction t with
+  | fn e Φ =>
+    calc e.fn.sub Subst.id'
+      _ = (e.sub (Subst.id'.keep _)).fn := rfl
+      _ = (e.sub Subst.id').fn := by rw [id_keep_eq_id]
+      _ = e.fn := by rw [Φ]
+  | var | true | false | zero => rfl
+  | succ e Φ | pred e Φ | zero? e Φ | fix e Φ => exact congrArg _ Φ
+  | app f a Φf Φa => exact congrArg2 _ Φf Φa
+  | cond s t f Φs Φt Φf => apply congrArg3 _ Φs Φt Φf
+
+def cx_eq_cons {Γ Δ : Cx} (p : Γ = Δ) (υ : Ty) : Γ ∷ υ = Δ ∷ υ := by
+  rw [p]
+
+def Var.tr_cx_z
+  (h : Γ ∷ υ = Δ ∷ υ) : (Var.z).tr_cx h = Var.z := by
+  cases h with | refl => rfl
+
+def Var.tr_cx_s
+  (h : Γ = Δ) : (Var.s τ x).tr_cx (cx_eq_cons h υ) = Var.s τ (x.tr_cx h) := by
+  cases h with | refl => rfl
+
+def keep_tr_cx
+  : (Ren.keep fun _ x ↦ x.tr_cx h : Ren (Γ ∷ υ) (Δ ∷ υ)) = fun _ x ↦ x.tr_cx (cx_eq_cons h υ) := by
+  funext τ x
+  induction h with | refl => cases x with | z | s => rfl
+
+-- NOTE: The signature of this lemma betrays the horror within.
+def sub_ren_exchange {t : Γ ⊢ τ} : ∀ {Δ} Δ' {Γ₀ Γ₁ : Cx} (h : Γ = Γ₀.append Δ') {σ : Subst Γ₀ Γ₁} {τ'}
+    (r : ∀ {Γ}, Ren (Γ.append (Δ.append Δ')) ((Γ ∷ τ').append (Δ.append Δ'))),
+    (∀ ν (x : Var Γ ν),
+      (σ.keeps'          (Δ.append Δ') ν      (((Ren.weaks Δ).keeps Δ' ν (x.tr_cx h)).tr_cx (Cx.append_append_eq Γ₀ Δ Δ'))).ren r
+    = (σ.keep τ').keeps' (Δ.append Δ') ν (r ν (((Ren.weaks Δ).keeps Δ' ν (x.tr_cx h)).tr_cx (Cx.append_append_eq Γ₀ Δ Δ'))))
+  → ((((t.tr_cx h).ren ((Ren.weaks Δ).keeps Δ')).tr_cx (Cx.append_append_eq Γ₀ Δ Δ')).sub (σ.keeps' (Δ.append Δ'))).ren r
+    = ((((t.tr_cx h).ren ((Ren.weaks Δ).keeps Δ')).tr_cx (Cx.append_append_eq Γ₀ Δ Δ')).ren r).sub ((σ.keep τ').keeps' (Δ.append Δ'))
+  := by
+  induction t with
+  | var υ x =>
+    intro Δ Δ' Γ₀ Γ₁ h σ τ' r lem
+    calc (σ.keeps' (Δ.append Δ') υ (((Ren.weaks Δ).keeps Δ' υ (x.tr_cx h)).tr_cx (Cx.append_append_eq Γ₀ Δ Δ'))).ren r
+      _ = (σ.keep τ').keeps' (Δ.append Δ') υ (r υ (((Ren.weaks Δ).keeps Δ' υ (x.tr_cx h)).tr_cx (Cx.append_append_eq Γ₀ Δ Δ')))
+      := by rw [lem]
+  | @fn Γ' υ τ e Φ =>
+    -- WARNING: Only suffering awaits.
+    intro Δ Δ' Γ₀ Γ₁ h σ τ' r lem
+    have lemₑ : ∀ (ν : Ty) (x : Var (Γ' ∷ υ) ν),
+      (σ.keeps'          (Δ.append (Δ' ∷ υ)) ν           (((Ren.weaks Δ).keeps (Δ' ∷ υ) ν (x.tr_cx (cx_eq_cons h υ))).tr_cx (Cx.append_append_eq Γ₀ Δ (Δ' ∷ υ)))).ren r.keep =
+      (σ.keep τ').keeps' (Δ.append (Δ' ∷ υ)) ν (r.keep ν (((Ren.weaks Δ).keeps (Δ' ∷ υ) ν (x.tr_cx (cx_eq_cons h υ))).tr_cx (Cx.append_append_eq Γ₀ Δ (Δ' ∷ υ)))) := by {
+        intro ν x
+        cases x with
+        | z =>
+          rw [Var.tr_cx_z]
+          show (σ.keeps' (Δ.append (Δ' ∷ υ)) υ (Var.z.tr_cx _)).ren r.keep
+            = (σ.keep τ').keeps' (Δ.append (Δ' ∷ υ)) υ (r.keep υ (Var.z.tr_cx _))
+          rw [Var.tr_cx_z]
+          rfl
+        | s ν x =>
+          -- First, we hide the casts under the constructor, allowing computations to proceed.
+          show (σ.keeps'          (Δ.append (Δ' ∷ υ)) ν           (((Ren.weaks Δ).keeps (Δ' ∷ υ) ν ((Var.s ν x).tr_cx (cx_eq_cons h υ))).tr_cx (Cx.append_append_eq Γ₀ Δ (Δ' ∷ υ)))).ren r.keep
+             = (σ.keep τ').keeps' (Δ.append (Δ' ∷ υ)) ν (r.keep ν (((Ren.weaks Δ).keeps (Δ' ∷ υ) ν ((Var.s ν x).tr_cx (cx_eq_cons h υ))).tr_cx (Cx.append_append_eq Γ₀ Δ (Δ' ∷ υ))))
+          rw [Var.tr_cx_s h]
+          show (σ.keeps'          (Δ.append (Δ' ∷ υ)) ν           ((Var.s ν ((Ren.weaks Δ).keeps Δ' ν (x.tr_cx h))).tr_cx (cx_eq_cons (Cx.append_append_eq Γ₀ Δ Δ') υ))).ren r.keep
+             = (σ.keep τ').keeps' (Δ.append (Δ' ∷ υ)) ν (r.keep ν ((Var.s ν ((Ren.weaks Δ).keeps Δ' ν (x.tr_cx h))).tr_cx (cx_eq_cons (Cx.append_append_eq Γ₀ Δ Δ') υ)))
+          rw [Var.tr_cx_s (Cx.append_append_eq Γ₀ Δ Δ')]
+          let y := (((Ren.weaks Δ).keeps Δ' ν (x.tr_cx h)).tr_cx (Cx.append_append_eq Γ₀ Δ Δ'))
+          let lem_x :
+            (σ.keeps' (Δ.append Δ') ν y).ren r = (σ.keep τ').keeps' (Δ.append Δ') ν (r ν y)
+            := lem ν x
+          -- To understand what's going on below, it's helpful to draw the components of the equation as a
+          -- diagram of context morphisms. The proof then follows by dissecting the diagram and proving its -- component equalities.
+          calc   (σ.keeps' (Δ.append (Δ' ∷ υ)) ν (Var.s ν y)).ren r.keep
+             _ = ((σ.keeps' (Δ.append Δ') ν y).ren Ren.weak).ren r.keep
+              := rfl
+             _ = (σ.keeps' (Δ.append Δ') ν y).ren (Ren.weak ⬝ r.keep)
+              := by rw [ren_trans_eq]
+             _ = (σ.keeps' (Δ.append Δ') ν y).ren (r ⬝ Ren.weak)
+              := by rw [Ren.weak_after_eq]
+             _ = ((σ.keeps' (Δ.append Δ') ν y).ren r).ren Ren.weak
+              := by rw [ren_trans_eq]
+             _ = ((σ.keep τ').keeps' (Δ.append Δ') ν (r ν y)).ren Ren.weak
+              := by rw [lem_x]
+             _ = (σ.keep τ').keeps' (Δ.append (Δ' ∷ υ)) ν (r.keep ν (Var.s ν y))
+              := rfl
+      }
+    -- TODO: Clean this up.
+    calc (((((e.fn).tr_cx h).ren ((Ren.weaks Δ).keeps Δ')).tr_cx (Cx.append_append_eq Γ₀ Δ Δ')).sub (σ.keeps' (Δ.append Δ'))).ren r
+    _ = (((((e.ren (Ren.keep fun _ x ↦ x.tr_cx h)).ren ((Ren.weaks Δ).keeps Δ').keep).ren (Ren.keep fun _ x ↦ x.tr_cx (Cx.append_append_eq Γ₀ Δ Δ'))).sub ((σ.keeps' (Δ.append Δ')).keep υ)).ren r.keep).fn
+      := rfl
+    _ = (((((e.ren (fun _ x ↦ x.tr_cx (cx_eq_cons h υ))).ren ((Ren.weaks Δ).keeps Δ').keep).ren (fun _ x ↦ x.tr_cx (cx_eq_cons (Cx.append_append_eq Γ₀ Δ Δ') υ))).sub ((σ.keeps' (Δ.append Δ')).keep υ)).ren r.keep).fn
+      := by rw [keep_tr_cx, keep_tr_cx]
+    _ = (((((e.tr_cx (cx_eq_cons h υ)).ren ((Ren.weaks Δ).keeps (Δ' ∷ υ))).tr_cx (Cx.append_append_eq Γ₀ Δ (Δ' ∷ υ))).sub ((σ.keeps' (Δ.append Δ')).keep υ)).ren r.keep).fn
+      := rfl
+    _ = (((((e.tr_cx (cx_eq_cons h υ)).ren ((Ren.weaks Δ).keeps (Δ' ∷ υ))).tr_cx (Cx.append_append_eq Γ₀ Δ (Δ' ∷ υ))).sub (σ.keeps' (Δ.append Δ' ∷ υ))).ren r.keep).fn
+      := by rw [Subst.keeps_keep_eq_keep]
+    _ = (((((e.tr_cx (cx_eq_cons h υ)).ren ((Ren.weaks Δ).keeps (Δ' ∷ υ))).tr_cx (Cx.append_append_eq Γ₀ Δ (Δ' ∷ υ))).sub (σ.keeps' (Δ.append (Δ' ∷ υ)))).ren r.keep).fn
+      := rfl
+    _ = (((((e.tr_cx (cx_eq_cons h υ)).ren ((Ren.weaks Δ).keeps (Δ' ∷ υ))).tr_cx (Cx.append_append_eq Γ₀ Δ (Δ' ∷ υ))).ren r.keep).sub ((σ.keep τ').keeps' (Δ.append (Δ' ∷ υ)))).fn
+      := by {
+        congr
+        apply Φ (Δ' ∷ υ) (cx_eq_cons h υ) r.keep lemₑ
+      }
+    _ = (((((e.ren (fun _ x ↦ x.tr_cx (cx_eq_cons h υ))).ren (((Ren.weaks Δ).keeps Δ').keep)).ren (fun _ x ↦ x.tr_cx (cx_eq_cons (Cx.append_append_eq Γ₀ Δ Δ') υ))).ren r.keep).sub (((σ.keep τ').keeps' (Δ.append Δ')).keep υ)).fn
+      := rfl
+    _ = (((((e.ren (Ren.keep fun _ x ↦ x.tr_cx h)).ren (((Ren.weaks Δ).keeps Δ').keep)).ren (Ren.keep fun _ x ↦ x.tr_cx (Cx.append_append_eq Γ₀ Δ Δ'))).ren r.keep).sub (((σ.keep τ').keeps' (Δ.append Δ')).keep υ)).fn
+      := by rw [keep_tr_cx, keep_tr_cx]
+    _ = (((((e.fn).tr_cx h).ren ((Ren.weaks Δ).keeps Δ')).tr_cx (Cx.append_append_eq Γ₀ Δ Δ')).ren r).sub ((σ.keep τ').keeps' (Δ.append Δ'))
+      := rfl
+  | true | false | zero => intros; rfl
+  | succ e Φ | pred e Φ | zero? e Φ | fix e Φ =>
+    intro _ _ _ _ _ _ _ r lem
+    exact congrArg _ (Φ _ _ r lem)
+  | app f a Φf Φa =>
+    intro _ _ _ _ _ _ _ r lem
+    exact congrArg2 _ (Φf _ _ r lem) (Φa _ _ r lem)
+  | cond s t f Φs Φt Φf =>
+    intro _ _ _ _ _ _ _ r lem
+    exact congrArg3 _ (Φs _ _ r lem) (Φt _ _ r lem) (Φf _ _ r lem)
+
+def sub_weak_exchange {t : Γ₀ ⊢ τ} {σ : Subst Γ₀ Γ₁}  : (t.sub σ).ren .s = (t.ren .s).sub (σ.keep υ) := by
+    have p
+      : (((((t.tr_cx rfl).ren ((Ren.weaks Cx.nil).keeps Cx.nil)).tr_cx rfl).sub (σ.keeps' (Cx.nil.append Cx.nil))).ren .s)
+      = ((((t.tr_cx rfl).ren ((Ren.weaks Cx.nil).keeps Cx.nil)).tr_cx rfl).ren .s).sub ((σ.keep υ).keeps' (Cx.nil.append Cx.nil))
+      := @sub_ren_exchange Γ₀ τ t Cx.nil Cx.nil Γ₀ Γ₁ rfl σ υ .s (fun ν x ↦ rfl)
+    rw [Tm.tr_cx_rfl, Tm.tr_cx_rfl] at p
+    change ((t.ren Ren.id').sub σ).ren .s = ((t.ren Ren.id').ren .s).sub (σ.keep υ) at p
+    rw [Tm.ren_id] at p
+    exact p
+
+def trans_keep_eq_id {σ₀₁ : Subst Γ₀ Γ₁} {σ₁₂ : Subst Γ₁ Γ₂} : (σ₀₁ ⬝ σ₁₂).keep τ = (σ₀₁.keep τ) ⬝ (σ₁₂.keep τ) := by
+  funext υ x
+  cases x with
+  | z => calc Var.z.tm = Var.z.tm := rfl
+  | s υ x =>
+    show ((σ₀₁ υ x).sub σ₁₂).ren .s = ((σ₀₁ υ x).ren .s).sub (σ₁₂.keep τ)
+    exact sub_weak_exchange
+
+def sub_trans_eq {t : Γ₀ ⊢ τ}
+  : ∀ {Γ₁ Γ₂} {σ₀₁ : Subst Γ₀ Γ₁} {σ₁₂ : Subst Γ₁ Γ₂}, t.sub (σ₀₁ ⬝ σ₁₂) = (t.sub σ₀₁).sub σ₁₂ := by
+  induction t with
+  | @fn _ τ υ e Φ =>
+    intro _ _ σ₀₁ σ₁₂
+    calc e.fn.sub (σ₀₁ ⬝ σ₁₂)
+      _ = (e.sub ((σ₀₁ ⬝ σ₁₂).keep τ)).fn := rfl
+      _ = (e.sub (σ₀₁.keep τ ⬝ σ₁₂.keep τ)).fn := by rw [trans_keep_eq_id]
+      _ = ((e.sub (σ₀₁.keep τ)).sub (σ₁₂.keep τ)).fn := by rw [Φ]
+      _ = (e.fn.sub σ₀₁).sub σ₁₂ := rfl
+  | var | true | false | zero => intros; rfl
+  | succ e Φ | pred e Φ | zero? e Φ | fix e Φ => exact congrArg _ Φ
+  | app f a Φf Φa => exact congrArg2 _ Φf Φa
+  | cond s t f Φs Φt Φf => exact congrArg3 _ Φs Φt Φf
+
+def sub_amend_keep_eq {r : Ren Γ₀ Γ₁} {σ : Subst Γ₁ Γ₂}
+  : (σ.amend r).keep τ = ((σ.keep τ).amend r.keep) := by
+  funext τ x
+  cases x with
+  | z | s => rfl
+
+def sub_amend_eq {t : Γ₀ ⊢ τ}
+  : ∀ {Γ₁ Γ₂} {r : Ren Γ₀ Γ₁} {σ : Subst Γ₁ Γ₂}, (t.ren r).sub σ = t.sub (σ.amend r) := by
+  induction t with
+  | fn e Φ =>
+    intro _ _ r σ
+    calc (e.fn.ren r).sub σ
+      _ = (((e.ren r.keep).sub (σ.keep _)).fn) := rfl
+      _ = ((e.sub ((σ.keep _).amend r.keep)).fn) := by rw [Φ]
+      _ = ((e.sub ((σ.amend r).keep _)).fn) := by rw [sub_amend_keep_eq]
+      _ = e.fn.sub (σ.amend r) := rfl
+  | var | true | false | zero => intros; rfl
+  | succ e Φ | pred e Φ | zero? e Φ | fix e Φ => exact congrArg _ Φ
+  | app f a Φf Φa => exact congrArg2 _ Φf Φa
+  | cond s t f Φs Φt Φf => exact congrArg3 _ Φs Φt Φf
+
+def inst_amend_weak_eq_id : (Subst.inst a).amend .s = Subst.id' := by
+  funext τ x
+  cases x with | z | s => rfl
+
+def ren_weak_sub_inst_eq {t : Γ ⊢ τ} : (t.ren .s).sub (Subst.inst a) = t := by
+  calc (t.ren .s).sub (Subst.inst a)
+    _ = t.sub ((Subst.inst a).amend .s) := by rw [sub_amend_eq]
+    _ = t.sub (Subst.id')               := by rw [inst_amend_weak_eq_id]
+    _ = t                               := by rw [sub_id_eq]
+
+def sub_push_eq_keep_inst {σ : Subst  Γ Δ} {υ : Ty} {a : Δ ⊢ υ} : σ.push a = σ.keep υ ⬝ Subst.inst a := by
+  funext τ x
+  cases x with
+  | z => rfl
+  | s τ x =>
+    calc σ.push a τ x.s
+      _ = σ τ x := rfl
+      _ = ((σ τ x).ren .s).sub (Subst.inst a) := by rw [ren_weak_sub_inst_eq]
+      _ = (σ.keep υ ⬝ Subst.inst a) τ x.s     := rfl
