oPCF/Utility.lean
@@ -5,3 +5,15 @@ def Nat.zero? : Nat → Bool
 theorem Nat.pred_succ_id : Nat.pred ∘ Nat.succ = id := by
   apply funext
   exact Nat.pred_succ
+
+infix:100 " ⬝ " => Trans.trans
+
+theorem congrArg2
+  {α₀ : Sort u₀} {α₁ : Sort u₁} {β : Sort v} {a₀ a₀' : α₀} {a₁ a₁' : α₁}
+  (f : α₀ → α₁ → β) (h₀ : Eq a₀ a₀') (h₁ : Eq a₁ a₁') : Eq (f a₀ a₁) (f a₀' a₁')
+  := h₀ ▸ h₁ ▸ rfl
+
+theorem congrArg3
+  {α₀ : Sort u₀} {α₁ : Sort u₁} {α₂ : Sort u₂} {β : Sort v} {a₀ a₀' : α₀} {a₁ a₁' : α₁} {a₂ a₂' : α₂}
+  (f : α₀ → α₁ → α₂ → β) (h₀ : Eq a₀ a₀') (h₁ : Eq a₁ a₁') (h₂ : Eq a₂ a₂') : Eq (f a₀ a₁ a₂) (f a₀' a₁' a₂')
+  := h₀ ▸ h₁ ▸ h₂ ▸ rfl
